proofs/compiler/boolean-dependent-2026-09-25/unhandled-instance.lean
@@ -6,4 +6,3 @@ def booleanDependentMany (x y : UInt64) : UInt64 :=
     let inner := a == b || b == c
     if _h : outer && !inner then a + b * 3 - c else a - b * 5 + c
   f x y (x + 7)
-
